ulib/LowStar.Array.fsti
@@ -6,23 +6,35 @@ open FStar.HyperStack.ST
 module U32 = FStar.UInt32
 module P = LowStar.Permissions
 
+/// `LowStar.Array` is the new workhorse of Low*, as the base class for every memory-allocated object that can be extracted to C.
+/// An array `b` is conceptually defined as a portion of a memory unit returned by a `malloc` call:
+///
+/// ```
+/// [Memory contents]
+///        +                        b.idx      b.idx + b.length    b.max_length
+///        +                          ↓              ↓                  ↓
+///    b.content  <-  [---------------|++++++++++++++|------------------]
+///        +                                ↑
+///        +                as_seq b, as_perm_seq b (depends on b.pid)
+///  [End of memory]
+/// ```
+///
+/// Each cell of the array is modelled as an independent memory location. You can view the contents of `b` in two different ways:
+/// * `as_seq h b` gives you access to the values stored at memory address `b.content` in heap `h`;
+/// * `as_perm_seq h b` gives the state of the permissions `b` currently owns over the cells of the array.
+///
+/// Indeed, `LowStar.Array` arrays are managed by a permission system, allowing you to effectively track aliasing over the memory location
+/// covered by the array. The permission system rely on a permission identifier `pid` stored in `b.pid`. You can have two arrays `b1` and `b2` pointing to the same memory location and same portion of an array, but distinc since they have different `pid`s.
+///
+/// The invariant maintained by the permission system is that for every cell of `b.content`, the sum of all permissions belonging to all the `pid`s created so far is less than the value 1, which represents full permission. Since all write-related operations require full permission to be called, this invariant effectively enforces a Rust-like aliasing rule : only one mutable alias at a time.
+
+/// `LowStar.Array.Defs` contains the base definitions of the class, while `LowStar.Array.Modifies` defines the `modifies` clauses theory on which our dynamic frame style of memory safety relies upon. The rest of this file defines all the stateful operations allowed on arrays.
+
 include LowStar.Array.Defs
 include LowStar.Array.Modifies
 
-(*** Stateful operations implementing the ghost specifications ***)
 
-
-val index (#a:Type) (b:array a) (i:U32.t{U32.v i < vlength b})
-  : Stack a (requires fun h -> live h b)
-            (ensures fun h0 y h1 -> h0 == h1 /\ y == get h0 b (U32.v i))
-
-val upd (#a:Type) (b:array a) (i:U32.t{U32.v i < vlength b}) (v:a) : Stack unit
-  (requires fun h -> writeable_cell h b (U32.v i) /\ live h b)
-  (ensures fun h0 _ h1 ->  writeable_cell h1 b (U32.v i) /\
-    modifies (loc_array b) h0 h1 /\
-    as_seq h1 b == Seq.upd (as_seq h0 b) (U32.v i) v /\
-    as_perm_seq h1 b == as_perm_seq h0 b
-  )
+(**** Allocation and deallocation *)
 
 val alloc (#a:Type0) (init:a) (len:U32.t)
   : ST (array a)
@@ -34,15 +46,34 @@ val alloc (#a:Type0) (init:a) (len:U32.t)
          freeable b /\
          as_seq h1 b == Seq.create (U32.v len) init)
 
+
+/// As per the C semantics, you can only free the entire allocation unit returned to you by `malloc`. This behavior is enforced by the
+/// `freeable` predicate, which doesn't depend on the heap. `freeable b` morally means : "`b` is not a subarray". `freeable` is preserved by all the functions that don't split their argument spatially. Freeing also requires full permission.
 val free (#a: Type) (b: array a) : HST.ST unit
-  (requires (fun h0 -> writeable h0 b /\ live  h0 b /\ freeable b))
+  (requires (fun h0 -> writeable h0 b /\ live h0 b /\ freeable b))
   (ensures (fun h0 _ h1 ->
-    Map.domain (HS.get_hmap h1) `Set.equal` Map.domain (HS.get_hmap h0) /\
-    (HS.get_tip h1) == (HS.get_tip h0) /\
-    modifies (loc_array b) h0 h1 /\
-    HS.live_region h1 (frameOf b)
+    modifies (loc_array b) h0 h1
   ))
 
+(****  Reading and writing *)
+
+/// The read operation only requires the array to be live.
+val index (#a:Type) (b:array a) (i:U32.t{U32.v i < vlength b})
+  : Stack a (requires fun h -> live h b)
+            (ensures fun h0 y h1 -> h0 == h1 /\ y == get h0 b (U32.v i))
+
+/// But to update, you need the full permission on the cell you want to change.
+val upd (#a:Type) (b:array a) (i:U32.t{U32.v i < vlength b}) (v:a) : Stack unit
+  (requires fun h -> writeable_cell h b (U32.v i) /\ live h b)
+  (ensures fun h0 _ h1 ->  writeable_cell h1 b (U32.v i) /\
+    modifies (loc_array b) h0 h1 /\
+    as_seq h1 b == Seq.upd (as_seq h0 b) (U32.v i) v /\
+    as_perm_seq h1 b == as_perm_seq h0 b
+  )
+
+(**** Permissions management *)
+
+/// `share b` effectively allocates a new `pid` and a corresponding array `b1` for the array `b`. The new `b1` array will conceptually be a immutable reference to `b` with same contents. However `b1` is disjoint from `b`; that is compatible with the `modifies` clause because neither `b` or `b1` will have full permission in `h1`, so you cannot modify the contents (with `upd`) of either of the two buffers. Caution: `b` is affected by `share` and loses half of its permission; if you had full permission on `b` in `h0`, it is no longer the case in `h1`.
 val share (#a:Type0) (b:array a) : Stack (array a)
   (requires fun h0 -> live h0 b /\ vlength b > 0)
   (ensures fun h0 b' h1 ->
@@ -51,19 +82,27 @@ val share (#a:Type0) (b:array a) : Stack (array a)
     loc_disjoint (loc_array b) (loc_array b') /\
     as_seq h0 b == as_seq h1 b /\ // The values of the initial array are not modified
     as_seq h1 b' == as_seq h1 b /\ // The values of the new array are the same as the initial array
-    mergeable b b' /\
+    gatherable b b' /\
     fresh_loc (loc_array b') h0 h1 /\
+    (freeable b ==> freeable b') /\
     (forall (i:nat{i < vlength b}). {:pattern get_perm h1 b' i \/ get_perm h1 b i } // The permission gets split in two
       get_perm h1 b' i == P.half_permission (get_perm h0 b i) /\
       get_perm h1 b i == P.half_permission (get_perm h0 b i)
     ))
 
-val merge:
+/// `share` issues a `gatherable` predicate used to track equivalence classes of references to the same thing. As such it is transitive (with a additional disjointness requirement), as well as commutative.
+val gatherable_trans (#a: Type0) (b1 b2 b3: array a): Lemma
+  (requires (gatherable b1 b2 /\ gatherable b2 b3 /\ loc_disjoint (loc_array b1) (loc_array b3)))
+  (ensures (gatherable b1 b3))
+  [SMTPat [gatherable b1 b2; gatherable b2 b3; gatherable b1 b3]]
+
+/// Gather is the reciprocal operation of `share`. It has to be use if you want to regain full permission on an array that you shared previously. The precondition of `gather` requires you to prove that you are managing your permissions correcty, since the permissions of `b` and `b1` have to be addable.
+val gather:
   #a: Type ->
   b: array a ->
   b1: array a ->
   Stack unit (requires (fun h0 ->
-    mergeable b b1 /\
+    gatherable b b1 /\
     live h0 b /\ live h0 b1 /\
     (forall (i:nat{i < vlength b}). summable_permissions h0 b b1  )
   ))
@@ -75,37 +114,55 @@ val merge:
     modifies (loc_array b `loc_union` loc_array b1) h0 h1
   ))
 
+/// `move` implements a different permission management pattern than `share`. It effectively "deactivates" the current reference to the array by giving it permission 0 and transferring the old permission to a new fresh reference.
 val move:
   #a: Type ->
   b: array a ->
   Stack (array a) (requires (fun h0 ->
     live h0 b
   )) (ensures (fun h0 b' h1 ->
-    live h1 b' /\ mergeable b b' /\ modifies (loc_array b) h0 h1 /\
+    live h1 b' /\ gatherable b b' /\ modifies (loc_array b) h0 h1 /\
     loc_disjoint (loc_array b) (loc_array b') /\
     fresh_loc (loc_array b') h0 h1  /\
     (freeable b ==> freeable b') /\
-    (forall (b1: array a{mergeable b b1}). {:pattern mergeable b' b1} mergeable b b1) /\
     as_seq h0 b == as_seq h1 b' /\
     as_perm_seq h0 b == as_perm_seq h1 b'
   ))
 
+(**** Spatial decomposition *)
+
+/// Standard sub-array extraction. The `gsub` postcondition is instrumented with lemmas such that `sub b` acts like a narrower view on the array `b`. However, it does not infer disjointness between non-overlapping `sub` of the same array. For that, see the functions below.
+val sub:
+ #a:Type0 ->
+ b:array a ->
+ i:U32.t ->
+ len:U32.t{U32.v len > 0} ->
+  Stack (array a)
+    (requires (fun h ->
+      U32.v i + U32.v len <= vlength b /\ live h b
+    ))
+    (ensures (fun h y h' ->
+      h == h' /\ y == gsub b i len
+    ))
+
+/// `split b` decomposes into to parts `b1` and `b2` such that `b` is the concatenation of `b1` and `b2`. These two parts are disjoints, so that modifying them plays nicely with the `modifies` theory. While `b1` and `b2` are in scope, you cannot use `b` anymore since it has lost its liveness.
 val split:
   #a: Type ->
   b: array a ->
   idx: U32.t{ U32.v idx > 0 /\ U32.v idx < vlength b} ->
   Stack (array a & array a) (requires (fun h0 ->
     live h0 b
-  )) (ensures (fun h0 (b1, b2) h1 ->
-    is_split_into b (b1,b2) /\ live h1 b1 /\ live h1 b2 /\
+  )) (ensures (fun h0 bs h1 ->
+    is_split_into b (fst bs, snd bs) /\ live h1 (fst bs) /\ live h1 (snd bs) /\
     modifies loc_none h0 h1 /\
-    loc_disjoint (loc_array b1) (loc_array b2) /\
-    as_seq h1 b1 == Seq.slice (as_seq h0 b) 0 (U32.v idx) /\
-    as_seq h1 b2 == Seq.slice (as_seq h0 b) (U32.v idx) (vlength b) /\
-    as_perm_seq h1 b1 == Seq.slice (as_perm_seq h0 b) 0 (U32.v idx) /\
-    as_perm_seq h1 b2 == Seq.slice (as_perm_seq h0 b) (U32.v idx) (vlength b)
+    loc_disjoint (loc_array (fst bs)) (loc_array (snd bs)) /\
+    as_seq h1 (fst bs) == Seq.slice (as_seq h0 b) 0 (U32.v idx) /\
+    as_seq h1 (snd bs) == Seq.slice (as_seq h0 b) (U32.v idx) (vlength b) /\
+    as_perm_seq h1 (fst bs) == Seq.slice (as_perm_seq h0 b) 0 (U32.v idx) /\
+    as_perm_seq h1 (snd bs) == Seq.slice (as_perm_seq h0 b) (U32.v idx) (vlength b)
   ))
 
+/// `glue` is the reciprocal of `split` in the same way `gather` is the reciprocal of `share`. However, `glue` is less flexible than `gather` since you have to provide the original `b` from which `b1` and `b2` have been `split` from.
 val glue:
   #a: Type ->
   b: array a ->
